somewhat working tactic.

src/boolring_tactic.lean
@@ -12,7 +12,6 @@ lemma finset.inter_is_inf (α : Type) [decidable_eq α] (X Y : finset α) : X �
 lemma finset.union_is_sup (α : Type) [decidable_eq α] (X Y : finset α) : X ∪ Y = X ⊔ Y := rfl
 lemma finset.empt_is_bot (α : Type) [decidable_eq α] : (finset.has_emptyc.emptyc : finset α) = ⊥ := rfl
 lemma finset.subset_is_le (α : Type) [decidable_eq α] (X Y : finset α) : (X ⊆ Y) = (X ≤ Y) := rfl 
-lemma finset.univ_is_top (α : Type) [decidable_eq α] : (finset.univ : finset α) = ⊤ := 
 
 lemma set.union_is_sup (α : Type) (X Y : set α) : X ∪ Y = X ⊔ Y := rfl
 lemma set.inter_is_inf (α : Type) (X Y : set α) : X ∩ Y = X ⊓ Y := rfl
@@ -20,16 +19,78 @@ lemma set.empt_is_bot (α : Type) : (set.has_emptyc.emptyc : set α) = ⊥ := rf
 lemma set.univ_is_top (α : Type) : (set.univ : set α) = ⊤ := rfl 
 lemma set.subset_is_le (α : Type) (X Y : set α) : (X ⊆ Y) = (X ≤ Y) := rfl 
 
+lemma ne_is_not_eq {α : Type} [boolean_algebra α] {X Y : α} : (X ≠ Y) = ¬(X = Y) := rfl 
+
+
 meta def to_ring_eqn : tactic unit := do
 `[
-      try { simp only
-      [finset.inter_is_inf, finset.union_is_sup, finset.empt_is_bot, finset.subset_is_le] at *}, 
-      try {simp only 
-      [set.union_is_sup, set.inter_is_inf, set.empt_is_bot, set.univ_is_top, set.subset_is_le] at *}, 
-      try {simp only 
-      [top_to_ring, bot_to_ring, symm_diff_to_ring,diff_to_ring, compl_to_ring, le_to_ring] at *}, 
-      try {simp only [inf_to_ring, sup_to_ring] at *}
+  try {simp only
+  [finset.inter_is_inf, finset.union_is_sup, finset.empt_is_bot, finset.subset_is_le] at *}, 
+  try {simp only 
+  [set.union_is_sup, set.inter_is_inf, set.empt_is_bot, set.univ_is_top, set.subset_is_le] at *}, 
+  try {simp only 
+  [top_to_ring, bot_to_ring, symm_diff_to_ring,diff_to_ring, compl_to_ring, le_to_ring] at *}, 
+  try {simp only [inf_to_ring, sup_to_ring] at *},
+  try {simp only [ne_is_not_eq] at *},
+  try {rw [bring_to_left] at *}
 ]
+
+#check and
+
+lemma convert_ands {A B A' B' : Prop} :
+  A = A' → B = B' → (A ∧ B) = (A' ∧ B') :=
+begin
+  cc,
+end
+
+meta def get_proof_normalization : expr → tactic (expr × expr)
+| e := do
+  match e with 
+  | `(%%L ∧ %%R) := do
+    (pfLT, pfLE) <- get_proof_normalization L,
+    (pfRT, pfRE) <- get_proof_normalization R,
+    match (pfLT, pfRT) with
+    | (`(_ = %%newL), `(_ = %%newR)) := do
+      proof_type <- to_expr ``(%%e = (%%newL ∧ %%newR)),
+      proof_expr <- to_expr 
+        ``(convert_ands %%pfLE %%pfRE : 
+            %%proof_type),
+      return (proof_type, proof_expr)
+    | _ := fail "Not here"
+    end
+   | `(%%A = %%B) := do
+    proof_type <- to_expr ``(%%e = (%%A + %%B + 1 = 1)),
+    proof_expr <- to_expr ``(bring_to_left : %%proof_type),
+    return (proof_type, proof_expr)
+  | _ := fail "Not here"
+  end
+
+meta def normalize_target : tactic unit := do
+  texpr <- target,
+  name <- get_unused_name `Hnormal,
+  (newTargetExpr, proofTerm) <- get_proof_normalization texpr,
+  hypExpr <- assertv name newTargetExpr proofTerm,
+  rewrite_target hypExpr,
+  clear hypExpr,
+  return ()
+
+meta def find_splittable_hyp : tactic expr := do
+  hyps <- local_context,
+  hyps <- hyps.mfilter (fun hyp, 
+    (do `(%%A ∧ %%B) <- infer_type hyp,
+        return tt)
+    <|> return ff),
+  match hyps with
+  | (x :: xs) := return x
+  | [] := fail "No splittable hypothesis found"
+  end
+
+meta def split_hyps : tactic unit := do
+  repeat $ (do
+    hyp <- find_splittable_hyp,
+    trace_state,
+    cases hyp,
+    skip)
 
 ------------------------------ Normalization Tactics (in a free boolean algebra) -------------------------
 meta def ids_list : lean.parser (list name) := types.list_of ident
@@ -41,8 +102,6 @@ meta def list_with_idx {T : Type} : (list T) → nat -> list (nat × T)
 | (v :: vs) n := (n, v) :: list_with_idx vs (n + 1)
 
 meta def tactic.interactive.introduce_varmap_rewrite (vname : parse ident) (vars : parse ids_list) : tactic unit :=
-  -- TODO: maybe vars should be a list of exprs here?
-  -- Especially if we're getting a list of expressions from get_sets_in_expr
   do
     names <- vars.mmap (fun name, get_local name),
     («let» vname ``(vector _ %%(vars.length)) $ meta_build_vector (names.map to_pexpr)),
@@ -53,9 +112,11 @@ meta def tactic.interactive.introduce_varmap_rewrite (vname : parse ident) (vars
         do 
           vname_expr <- get_local vname,
           hname <- get_unused_name `Hv,
+          -- TODO: maybe clean this up with definev/assertv instead.
           («have» hname ``(%%name = _) ``(on_var %%vname_expr %%idx (by norm_num))),
           hname_expr <- get_local hname,
           tactic.try (rewrite_target hname_expr),
+          clear hname_expr,
           return ())
       (list_with_idx names 0),
     return ()
@@ -76,17 +137,8 @@ meta def get_sets_in_expr : expr → tactic (list name)
     do
       expr <- get_local pretty,
       ((do
-        `(finset _) <- tactic.infer_type expr, 
-        return [pretty])
-      <|>
-       (do
-        `(set _) <- tactic.infer_type expr,
-        return [pretty])
-      <|>
-       (do
         `(%%typ) <- tactic.infer_type expr,
-        boolalg_expr_to_find <- to_expr ``(boolean_algebra %%typ),
-        _ <- find_assumption boolalg_expr_to_find,
+        boolalg_hyp <- to_expr ``(infer_instance : boolean_algebra %%typ),
         return [pretty])
       <|>
         return [])
@@ -96,6 +148,31 @@ meta def get_sets_in_expr : expr → tactic (list name)
        return (l1 ++ l2)
   | _ := do return []
   end
+
+meta def assert_expr_is_boolalg (e : expr) : tactic unit :=
+do
+  typ <- tactic.infer_type e,
+  boolalg_hyp <- to_expr ``(infer_instance : boolean_algebra %%typ),
+  return ()
+  
+meta def is_boolalg_eqn : expr → tactic bool
+| e :=
+  ((do `(%%L = %%R) <- (infer_type e),
+    assert_expr_is_boolalg L,
+    assert_expr_is_boolalg R,
+    return tt)
+  <|>
+  (do `(%%L ≠ %%R) <- (infer_type e),
+    assert_expr_is_boolalg L,
+    assert_expr_is_boolalg R,
+    return tt)
+  <|>
+  (do `(¬ %%L = %%R) <- (infer_type e),
+    assert_expr_is_boolalg L,
+    assert_expr_is_boolalg R,
+    return tt)
+  <|>
+  (return ff))
 
 def keep_unique {T: Type}[decidable_eq T]: list T -> list T 
 | [] := []
@@ -127,22 +204,46 @@ they are sometimes dummy values. Use `tactic.infer_type` instead. -/
   The list of expressions are local constants and metavariables that the macro depends on.
   -/
 -- | expr.macro macro_def body := do return () 
-
 meta def dummy : tactic unit :=
   do tactic.trace "Hello World"
 
-meta def tactic.interactive.simplify_sets (extra_sets : (parse (optional ids_list))): tactic unit :=
-  do
-    -- TODO: actually check the goal is of the form of some boolalg equation
-    --       also -- do something about hypotheses...
-    -- Probably makes sense to automatically include sets mentioned in the goal, analogously to linarith 
+lemma switch_target {T : Type} [boolean_algebra T] (A B C : T):
+  (A = 1) → (A * B = A * C) → B = C :=
+  λ h1 h2, by {rw [h1,one_mul, one_mul] at h2, from h2}
+    
+-- expects that goal is conjunction of ring equations
+-- expects that assumptions are just ring equations
+meta def simplify_one_set (extra_sets : list name): tactic unit :=
+  do   
+    -- Convert to ring equations, and also
+    -- convert ring hypothesis to be of the form <eqn> = 1
+
+    -- TODO: gather sets from goals and hypothesis evntually
+    -- before we convert the goal as that's expensive.
+    timetac "rewrite to ring equation" $ to_ring_eqn,
+    normalize_target,
+    timetac "rewrite ∧ to ring equns" $ try `[apply no_inverses],
+    context <- tactic.local_context,
+    boolalg_hyps <- timetac "get boolalg hyp" $ context.mfilter is_boolalg_eqn,
+    -- Rewrite target to be Π (hypothesis) * original target
+    -- Clear original ring hypothesis as they are not needed anymore
+    tactic.timetac "rewrite target" $ boolalg_hyps.mmap
+      (fun (hyp : expr), do
+        `(%%Lh = 1) <- infer_type hyp,
+        `(%%Ltarget = %%Rtarget) <- target,
+        `[apply (switch_target %%Lh %%Ltarget %%Rtarget %%hyp)],
+        return ()
+      ),
+
+    -- Gather sets in the goal
     texpr <- target,
-    list_of_sets <- get_sets_in_expr texpr,
+    list_of_sets <- timetac "get set names" $ get_sets_in_expr texpr,
+    tactic.trace list_of_sets,
     vname <- get_unused_name `V,
     tactic.timetac "rewrite names" $ tactic.interactive.introduce_varmap_rewrite vname
-      (keep_unique $ list_of_sets ++ match extra_sets with | some l := l | none := [] end ),
+      (keep_unique $ list_of_sets ++ extra_sets),
     vname_expr <- get_local vname,
-    to_ring_eqn,
+
     -- Some goals are already discharged by this point, so everything else
     -- goes in a try block.
     tactic.timetac "final simp" $
@@ -153,3 +254,40 @@ meta def tactic.interactive.simplify_sets (extra_sets : (parse (optional ids_lis
                    ``(freealg.on_var %%vname_expr)].map simp_arg_type.expr)
                     list.nil loc.wildcard),
     tactic.timetac "evaluate ring stuff" $ tactic.try (refl)
+
+meta def split_goal (solver : tactic unit): tactic unit := do
+  texpr <- target,
+  match texpr with
+  | `(%%A ∨ %%B) := do
+    trace $ "splitting: " ++ (to_string A) ++ (to_string B),
+    (left >> split_goal <|> right >> split_goal)
+  | _ := solver
+  end
+
+meta def tactic.interactive.timed_simplify_sets 
+  (extra_sets : (parse (optional ids_list))): tactic unit :=
+    do timetac "simplify sets" $ simplify_one_set (match extra_sets with | some l := l | none := [] end)
+
+lemma fourlemma (T : Type) (A B C D : set T) : A ⊆ B → C ⊆ Bᶜ → D ⊆ Bᶜ → ((A ∩ C = ∅ ) ∧ (A ∩ D = ∅)):=
+begin
+  intros,
+  timed_simplify_sets,
+end
+
+--lemma fourtrans (T : Type) (A B C D : set T) : (A ⊆ B) → (B ⊆ C) → (C ⊆ D) → (A ⊆ D) :=
+--begin
+--  intros,
+--  timed_simplify_sets,
+--end
+
+--lemma dummylemma (T: Type) (X Y Z : set T) : (T = nat) → (X ⊆ Y) → (X ∩ Z) ⊆ (Y ∩ Z) :=
+--begin
+--  intros H1 H2,      
+--  simplify_sets,
+--end
+
+--lemma foo_alg2 (α : Type) (A: boolean_algebra α) (X Y Z P Q W: α): 
+--  (X ⊔ (Y ⊔ Z)) ⊔ ((W ⊓ P ⊓ Q)ᶜ ⊔ (P ⊔ W ⊔ Q)) = ⊤ :=
+--begin
+--  simplify_sets, 
+--end
